Setlec/Verify/SimIKnot.lean
@@ -67,7 +67,7 @@ theorem ISOK.insertWhnfCoreC {s : IState} (hs : ISOK env s)
     ISOK env { s with whnfCoreC := s.whnfCoreC.insert i j } := by
   refine ⟨hs.wf, hs.constTy, hs.constVal, hs.ruleRhs, ?_, hs.whnfC,
     hs.inferC, hs.annotC, hs.defeqC, hs.lsimp, hs.lnz, hs.eqv,
-    hs.ienv⟩
+    hs.ienv, hs.instC⟩
   intro i' j' hl
   simp only at hl
   rw [Std.HashMap.getElem?_insert] at hl
@@ -86,7 +86,7 @@ theorem ISOK.insertWhnfC {s : IState} (hs : ISOK env s)
     ISOK env { s with whnfC := s.whnfC.insert i j } := by
   refine ⟨hs.wf, hs.constTy, hs.constVal, hs.ruleRhs, hs.whnfCoreC, ?_,
     hs.inferC, hs.annotC, hs.defeqC, hs.lsimp, hs.lnz, hs.eqv,
-    hs.ienv⟩
+    hs.ienv, hs.instC⟩
   intro i' j' hl
   simp only at hl
   rw [Std.HashMap.getElem?_insert] at hl
@@ -106,7 +106,7 @@ theorem ISOK.insertInferC {s : IState} (hs : ISOK env s)
     ISOK env { s with inferC := s.inferC.insert i j } := by
   refine ⟨hs.wf, hs.constTy, hs.constVal, hs.ruleRhs, hs.whnfCoreC,
     hs.whnfC, ?_, hs.annotC, hs.defeqC, hs.lsimp, hs.lnz, hs.eqv,
-    hs.ienv⟩
+    hs.ienv, hs.instC⟩
   intro i' j' hl
   simp only at hl
   rw [Std.HashMap.getElem?_insert] at hl
@@ -126,7 +126,7 @@ theorem ISOK.insertAnnotC {s : IState} (hs : ISOK env s)
     ISOK env { s with annotC := s.annotC.insert i j } := by
   refine ⟨hs.wf, hs.constTy, hs.constVal, hs.ruleRhs, hs.whnfCoreC,
     hs.whnfC, hs.inferC, ?_, hs.defeqC, hs.lsimp, hs.lnz, hs.eqv,
-    hs.ienv⟩
+    hs.ienv, hs.instC⟩
   intro i' j' hl
   simp only at hl
   rw [Std.HashMap.getElem?_insert] at hl
@@ -146,7 +146,7 @@ theorem ISOK.insertDefeqC {s : IState} (hs : ISOK env s)
     ISOK env { s with defeqC := s.defeqC.insert (i, j) r } := by
   refine ⟨hs.wf, hs.constTy, hs.constVal, hs.ruleRhs, hs.whnfCoreC,
     hs.whnfC, hs.inferC, hs.annotC, ?_, hs.lsimp, hs.lnz, hs.eqv,
-    hs.ienv⟩
+    hs.ienv, hs.instC⟩
   intro i' j' r' hl
   simp only at hl
   rw [Std.HashMap.getElem?_insert] at hl
